prove a lemma for for-loop

LoL/MProp/HoareTriples.lean
@@ -5,7 +5,47 @@ universe u v w
 
 variable {m : Type u -> Type v} [Monad m] [LawfulMonad m] {α : Type u}
 variable {l : Type u} [Preorder l]
+
+section
 variable [MProp m l]
 
-def triple (pre : m PProp) (c : m α) (post : α -> m PProp) : Prop :=
-  MProp.μ pre ≤ liftM (n := Cont l) c (MProp.μ (m := m) ∘ post)
+def triple (pre : l) (c : m α) (post : α -> l) : Prop :=
+  pre ≤ liftM (n := Cont l) c post
+
+abbrev mtriple (pre : m PProp) (c : m α) (post : α -> m PProp) : Prop :=
+  triple (MProp.μ pre) c (MProp.μ (m := m) ∘ post)
+
+lemma mtriple_pure (pre : m PProp) (x : α) (post : α -> m PProp) :
+  MProp.μ pre ≤ MProp.μ (post x) ->
+  mtriple pre (pure x) post := by
+    intros h; rw [mtriple, triple]; simp [liftM, lift_pure]; apply h
+end
+
+variable [MPropOrdered m l]
+
+lemma mtriple_bind {β} (pre : m PProp) (x : m α) (cut : α -> m PProp)
+  (f : α -> m β) (post : β -> m PProp) :
+  mtriple pre x cut ->
+  (∀ y, mtriple (cut y) (f y) post) ->
+  mtriple pre (x >>= f) post := by
+    intros hcut hpost
+    simp [mtriple, triple, liftM, lift_bind]
+    apply le_trans; apply hcut
+    have h: monadLift x = MProp.lift x := by rfl
+    simp [h, Bind.bind];
+    apply Cont.monotone_lift; apply hpost
+
+theorem Triple.forIn_list {α β}
+  {xs : List α} {init : β} {f : α → β → m (ForInStep β)}
+  (inv : List α → β → m PProp)
+  (hstep : ∀ hd tl b,
+    mtriple
+      (inv (hd :: tl) b)
+      (f hd b)
+      (fun | .yield b' => inv tl b' | .done b' => inv [] b')) :
+  mtriple (inv xs init) (forIn xs init f) (inv []) := by
+    induction xs generalizing init
+    { apply mtriple_pure; simp }
+    simp only [List.forIn_cons]
+    apply mtriple_bind; apply hstep; intros y
+    cases y <;> simp <;> solve_by_elim [mtriple_pure, le_refl]
